LocallyNameless/STLC/Constants/Development.v
@@ -1,0 +1,151 @@
+From FormalSystems Require Export LocallyNameless.STLC.Constants.Confluence.
+
+Axiom Development : Tm -> Tm -> Prop.
+
+Axiom Development_spec :
+  forall t1 t2 t3 : Tm,
+    Development t1 t3 ->
+    ParallelStep t1 t2 -> ParallelStep t2 t3.
+
+Lemma confluent_ParallelStep :
+  forall t t' t1 t2 : Tm,
+    Development t t' ->
+    ParallelStep t t1 -> ParallelStep t t2 ->
+      ParallelStep t1 t' /\ ParallelStep t2 t'.
+Proof.
+  intros t t' t1 t2 Hd Hps1 Hps2.
+  now split; eapply Development_spec; eauto.
+Qed.
+
+Inductive ParallelMultiStep : Tm -> Tm -> Prop :=
+| ParallelMultiStep_refl :
+  forall (t : Tm),
+    lc t ->
+    ParallelMultiStep t t
+| ParallelMultiStep_step_trans :
+  forall (t1 t2 t3 : Tm),
+    ParallelStep t1 t2 ->
+    ParallelMultiStep t2 t3 ->
+    ParallelMultiStep t1 t3.
+
+#[export] Hint Constructors ParallelMultiStep : core.
+
+Require Import Coq.Classes.RelationClasses.
+
+#[export] Instance Transitive_ParallelMultiStep : Transitive ParallelMultiStep.
+Proof.
+  now induction 1; eauto.
+Qed.
+
+Lemma lc_ParallelMultiStep_l :
+  forall t t' : Tm,
+    ParallelMultiStep t t' -> lc t.
+Proof.
+  now induction 1; eauto.
+Qed.
+
+Lemma lc_ParallelMultiStep_r :
+  forall t t' : Tm,
+    ParallelMultiStep t t' -> lc t'.
+Proof.
+  now induction 1; eauto.
+Qed.
+
+Lemma ParallelMultiStep_ParallelStep :
+  forall t1 t2 : Tm,
+    ParallelStep t1 t2 -> ParallelMultiStep t1 t2.
+Proof.
+  now eauto.
+Qed.
+
+#[export] Hint Resolve
+  lc_ParallelMultiStep_l lc_ParallelMultiStep_r
+  ParallelMultiStep_ParallelStep
+    : core.
+
+Lemma ParallelMultiStep_app_l :
+  forall t1 t1' t2 : Tm,
+    ParallelMultiStep t1 t1' ->
+    lc t2 ->
+      ParallelMultiStep (app t1 t2) (app t1' t2).
+Proof.
+  now induction 1; eauto.
+Qed.
+
+Lemma ParallelMultiStep_app_r :
+  forall t1 t2 t2' : Tm,
+    lc t1 ->
+    ParallelMultiStep t2 t2' ->
+      ParallelMultiStep (app t1 t2) (app t1 t2').
+Proof.
+  now induction 2; eauto.
+Qed.
+
+Lemma ParallelMultiStep_app :
+  forall t1 t1' t2 t2' : Tm,
+    ParallelMultiStep t1 t1' ->
+    ParallelMultiStep t2 t2' ->
+      ParallelMultiStep (app t1 t2) (app t1' t2').
+Proof.
+  intros.
+  transitivity (app t1' t2).
+  - now apply ParallelMultiStep_app_l; eauto.
+  - now apply ParallelMultiStep_app_r; eauto.
+Qed.
+
+#[export] Hint Resolve
+  ParallelMultiStep_app_l ParallelMultiStep_app_r ParallelMultiStep_app
+    : core.
+
+Lemma MultiStep_ParallelMultiStep :
+  forall t1 t2 : Tm,
+    MultiStep t1 t2 <-> ParallelMultiStep t1 t2.
+Proof.
+  split.
+  - now induction 1; eauto.
+  - induction 1; [now eauto |].
+    now transitivity t2; eauto.
+Qed.
+
+Lemma confluent_ParallelStep_ParallelMultiStep :
+  forall t t1 t2 : Tm,
+    ParallelStep t t1 -> ParallelMultiStep t t2 ->
+      exists t3 : Tm, ParallelMultiStep t1 t3 /\ ParallelMultiStep t2 t3.
+Proof.
+  intros t t1 t2 H1 H2; revert t1 H1.
+  induction H2; intros; [now exists t1; eauto |].
+  edestruct (IHParallelMultiStep (Development t1)) as [t4 [IH1 IH2] ].
+  - now apply Development_spec.
+  - exists t4; split; [| easy].
+    transitivity (Development t1); [| easy].
+    now apply ParallelMultiStep_ParallelStep, Development_spec.
+Qed.
+
+Lemma confluent_ParallelMultiStep :
+  forall t t1 t2 : Tm,
+    ParallelMultiStep t t1 -> ParallelMultiStep t t2 ->
+      exists t3 : Tm, ParallelMultiStep t1 t3 /\ ParallelMultiStep t2 t3.
+Proof.
+  intros t t1 t2 H1 H2; revert t2 H2.
+  induction H1; intros; [now exists t2; eauto |].
+  destruct (confluent_ParallelStep_ParallelMultiStep _ _ _ H H2) as [t4 [H24 H04] ].
+  edestruct (IHParallelMultiStep _ H24) as [t5 [H35 H45] ].
+  exists t5; split; [easy |].
+  now transitivity t4.
+Qed.
+
+Lemma confluent_Step :
+  forall t t1 t2 : Tm,
+    MultiStep t t1 -> MultiStep t t2 ->
+      exists t3 : Tm, MultiStep t1 t3 /\ MultiStep t2 t3.
+Proof.
+  setoid_rewrite MultiStep_ParallelMultiStep.
+  now apply confluent_ParallelMultiStep.
+Qed.
+
+Print Assumptions confluent_Step.
+Print Assumptions ParallelStep_refl.
+Print Assumptions MultiStep_abs.
+Print Assumptions confluent_Step.
+
+
